IrisITree/IrisITree/Effects/Heap.lean
@@ -1,7 +1,162 @@
 module
 
+public import IrisITree.Effects.State
+public import IrisITree.Effects.Demonic
+public import IrisITree.Effects.Fail
+public import ITree.Effects.Heap
+public import Iris.BI.BigOp.BigSepList
+public import Iris.Instances.Lib.GhostMap
+public import Iris.Instances.Lib.Invariants
+public import Iris.Std.HeapInstances
+
 @[expose] public section
 
 -- A heap, represented as a [gmap] of [option val]s, with [None] representing deallocated locations.
 
 namespace IrisITree.Effects
+
+open Iris BI ITree Effects Core
+
+-- TODO: Why can’t we make this universe-polymorphic? `Loc` and `Val` should have type `Type _`
+-- The restriction seems to come from `GhostMapG`; More concretely, `constOF` is too conservative.
+class heapHGpreS (GF : BundledGFunctors) (Loc Val : Type)
+    [Ord Loc] [Std.TransOrd Loc] [Std.LawfulEqOrd Loc] where
+  heapH_ghost_varG : GhostMapG GF Loc (Option Val) (Std.ExtTreeMap Loc · compare)
+
+attribute [reducible, instance] heapHGpreS.heapH_ghost_varG
+
+class heapHGS (GF : BundledGFunctors) (Loc Val : Type)
+    [Ord Loc] [Std.TransOrd Loc] [Std.LawfulEqOrd Loc] where
+  heapH_inG : heapHGpreS GF Loc Val
+  heapH_heap_name : GName
+  heapH_inv_name_postfix : String
+
+attribute [reducible, instance] heapHGS.heapH_inG
+
+def heapH_inv_name {GF : BundledGFunctors} {Loc Val : Type}
+    [Ord Loc] [Std.TransOrd Loc] [Std.LawfulEqOrd Loc]
+    [G : heapHGS GF Loc Val] : Namespace :=
+  (nroot.@"heapH").@G.heapH_inv_name_postfix
+
+def pointsto {GF : BundledGFunctors} {Loc Val : Type}
+    [Ord Loc] [Std.TransOrd Loc] [Std.LawfulEqOrd Loc]
+    [G : heapHGS GF Loc Val] (l : Loc) (v : Option Val) (dq : DFrac) : IProp GF :=
+  ghost_map_elem (G.heapH_heap_name) dq l v
+
+notation:50 l:50 " ↦? " v:50 => pointsto l v (DFrac.own 1)
+notation:50 l:50 " ↦{" dq "}? " v:50 => pointsto l v dq
+notation:50 l:50 " ↦ " v:50 => pointsto l (some v) (DFrac.own 1)
+notation:50 l:50 " ↦{" dq "} " v:50 => pointsto l (some v) dq
+
+section handler
+
+variable {GF : BundledGFunctors} {hlc : HasLC} [InvGS_gen hlc GF]
+variable {Loc Val : Type} [Ord Loc] [Std.TransOrd Loc] [Std.LawfulEqOrd Loc]
+variable [G : heapHGS GF Loc Val]
+
+def heap_inv : IProp GF :=
+  inv (heapH_inv_name (G := G)) iprop(
+    ∃ σ : heapE.T Loc Val,
+      ghost_map_auth (GF := GF) (K := Loc) (V := Option Val)
+        (H := (Std.ExtTreeMap Loc · compare))
+        G.heapH_heap_name
+        (DFrac.own (Qp.half (1 : Qp))) σ
+  )
+
+def stateInterp_heap (σ : heapE.T Loc Val) : IProp GF := iprop(
+  ghost_map_auth (GF := GF) (K := Loc) (V := Option Val)
+      (H := (Std.ExtTreeMap Loc · compare))
+      G.heapH_heap_name
+      (DFrac.own (Qp.half (1 : Qp))) σ ∧
+    heap_inv (G := G)
+)
+
+def heapH : IHandler (IProp GF) (heapE Loc Val) :=
+  stateH stateInterp_heap
+
+end handler
+
+section wpi_rules
+
+variable {GF : BundledGFunctors} {hlc : HasLC} [InvGS_gen hlc GF]
+variable {Loc Val : Type} [Ord Loc] [Std.TransOrd Loc] [Std.LawfulEqOrd Loc]
+variable [heapHGS GF Loc Val]
+variable {E : Effect} {H : IHandler (IProp GF) E}
+variable [heapE Loc Val -< E]
+variable [InH (heapH (GF := GF) (hlc := hlc) (Loc := Loc) (Val := Val)) H]
+
+theorem wpi_load_opt M (l : Loc) (v : Val) (dq : DFrac)
+    (Φ : Option Val → IProp GF) :
+    ↑(heapH_inv_name (GF := GF) (Loc := Loc) (Val := Val)) ⊆ M →
+    pointsto (GF := GF) (Loc := Loc) (Val := Val) l (some v) dq -∗
+    (pointsto (GF := GF) (Loc := Loc) (Val := Val) l (some v) dq -∗ Φ (some v)) -∗
+    WPi (HeapE.load? (E := E) (Loc := Loc) (Val := Val) l) @> H; M {{ Φ }} := by
+  sorry
+
+theorem wpi_storeOpt M (l : Loc) (v v' : Option Val)
+    (Φ : Option Val → IProp GF) :
+    ↑(heapH_inv_name (GF := GF) (Loc := Loc) (Val := Val)) ⊆ M →
+    pointsto (GF := GF) (Loc := Loc) (Val := Val) l v (DFrac.own (1 : Qp)) -∗
+    (pointsto (GF := GF) (Loc := Loc) (Val := Val) l v' (DFrac.own (1 : Qp)) -∗ Φ v) -∗
+    WPi (HeapE.storeOpt (E := E) (Loc := Loc) (Val := Val) l v') @> H; M {{ Φ }} := by
+  sorry
+
+theorem wpi_store M (l : Loc) (v : Option Val) (v' : Val)
+    (Φ : Option Val → IProp GF) :
+    ↑(heapH_inv_name (GF := GF) (Loc := Loc) (Val := Val)) ⊆ M →
+    pointsto (GF := GF) (Loc := Loc) (Val := Val) l v (DFrac.own (1 : Qp)) -∗
+    (pointsto (GF := GF) (Loc := Loc) (Val := Val) l (some v') (DFrac.own (1 : Qp)) -∗ Φ v) -∗
+    WPi (HeapE.store? (E := E) (Loc := Loc) (Val := Val) l v') @> H; M {{ Φ }} := by
+  sorry
+
+section fail
+
+variable [failE -< E] [InH (failH (PROP := IProp GF)) H]
+
+theorem wpi_load_bang M (l : Loc) (v : Val) (dq : DFrac)
+    (Φ : Val → IProp GF) :
+    ↑(heapH_inv_name (GF := GF) (Loc := Loc) (Val := Val)) ⊆ M →
+    pointsto (GF := GF) (Loc := Loc) (Val := Val) l (some v) dq -∗
+    (pointsto (GF := GF) (Loc := Loc) (Val := Val) l (some v) dq -∗ Φ v) -∗
+    WPi (HeapE.load! (E := E) (Loc := Loc) (Val := Val) l) @> H; M {{ Φ }} := by
+  sorry
+
+theorem wpi_store_bang M (l : Loc) (v v' : Val) (Φ : Val → IProp GF) :
+    ↑(heapH_inv_name (GF := GF) (Loc := Loc) (Val := Val)) ⊆ M →
+    pointsto (GF := GF) (Loc := Loc) (Val := Val) l (some v) (DFrac.own (1 : Qp)) -∗
+    (pointsto (GF := GF) (Loc := Loc) (Val := Val) l (some v') (DFrac.own (1 : Qp)) -∗ Φ v) -∗
+    WPi (HeapE.store! (E := E) (Loc := Loc) (Val := Val) l v') @> H; M {{ Φ }} := by
+  sorry
+
+end fail
+
+section alloc
+
+variable [demonicE Loc -< E] [InH (demonicH (PROP := IProp GF) Loc) H]
+variable [Zero Loc] [HAdd Loc Int Loc]
+
+theorem wpi_allocN M (n : Nat) (v : Val)
+    (hle : ∀ (l : Loc) (m : Nat), ¬(compare (l + (1 : Int) + (m : Int)) l).isLE = true)
+    (Φ : Loc → IProp GF) :
+    ↑(heapH_inv_name (GF := GF) (Loc := Loc) (Val := Val)) ⊆ M →
+    (∀ l : Loc,
+      bigSepL (fun _ (i : Nat) =>
+        pointsto (GF := GF) (Loc := Loc) (Val := Val)
+          (l + (i : Int)) (some v) (DFrac.own (1 : Qp))) (List.range n) -∗ Φ l) -∗
+    WPi (HeapE.allocN (E := E) (Loc := Loc) (Val := Val) n v hle) @> H; M {{ Φ }} := by
+  sorry
+
+theorem wpi_alloc M (v : Val)
+    (hle : ∀ (l : Loc) (m : Nat), ¬(compare (l + (1 : Int) + (m : Int)) l).isLE = true)
+    (Φ : Loc → IProp GF) :
+    ↑(heapH_inv_name (GF := GF) (Loc := Loc) (Val := Val)) ⊆ M →
+    (∀ l : Loc,
+      pointsto (GF := GF) (Loc := Loc) (Val := Val) l (some v) (DFrac.own (1 : Qp)) -∗ Φ l) -∗
+    WPi (HeapE.alloc (E := E) (Loc := Loc) (Val := Val) v hle) @> H; M {{ Φ }} := by
+  sorry
+
+end alloc
+
+end wpi_rules
+
+end IrisITree.Effects
